\bigskip
\section*{RÃ©ponses}

\begin{reponse}{2.1}
    \begin{inparaenum}
      \stepcounter{enumi}
      \stepcounter{enumi}
    \item $\hat{\beta}_0=66.44882$ et $\hat{\beta}_1=-0.8407468$
    \item $\hat{Y}_1 = 11,80, \hat{Y}_2 = 30,30, \hat{Y}_3 = 29,46,
      \hat{Y}_4 = 16,84, \hat{Y}_5 = 16,00, \hat{Y}_6 = 24,41,
      \hat{Y}_7 = 22,73, \hat{Y}_8 = 34,50, \hat{Y}_9 = 31,14,
      \hat{Y}_{10} = 32,82$
    \end{inparaenum}
  
\end{reponse}
\begin{reponse}{2.2}
    \begin{inparaenum}
    \item $\hat{\beta}_0=7$ et $\hat{\beta}_1=-0,5$
    \item SST = 14, SSR = 7, SSE = 7, MSR = 7, MSE = 7/6, $F$ = 6, $R^2$ = 0,5
    \end{inparaenum}
  
\end{reponse}
\begin{reponse}{2.3}
    \begin{inparaenum}
      \stepcounter{enumi}
    \item
      $\hat{\beta}_0 = -87,5167$
      et
      $\hat{\beta}_1 = 3,45$
      \stepcounter{enumi}
    \item $R^2 = 0,991$
    \item
      $\SSR = 3332,7$
      $\SSE = 30,23$ et
      $\SST = 3362,93$
    \end{inparaenum}
  
\end{reponse}
\begin{reponse}{2.5}
    $\hat{\beta}_0 = \bar{Y} - \hat{\beta}_1 (n + 1)/2$,
    $\hat{\beta}_1 = (12 \sum_{t = 0}^n t Y_t - 6 n (n + 1)
    \bar{Y})/(n (n^2 - 1)$
  
\end{reponse}
\begin{reponse}{2.6}
    \begin{inparaenum}
    \item $\hat{\beta}= \sum_{t = 1}^n X_t Y_t/\sum_{t = 1}^n X_t^2$
      \stepcounter{enumi}
    \item $\var{\hat{\beta}} = \sigma^2/\sum_{t = 1}^n X_t^2$
    \end{inparaenum}
  
\end{reponse}
\begin{reponse}{2.9}
    \begin{enumerate}
    \item $\hat{\beta}_1^\prime = (b/d) \hat{\beta}_1$
    \end{enumerate}
  
\end{reponse}
\begin{reponse}{2.11}
    $\beta_1 \in \hat{\beta}_1 \pm z_{\alpha/2} \sigma
    \left( \sum_{t=1}^n (X_t - \bar{X})^2 \right)^{-1/2}$
  
\end{reponse}
\begin{reponse}{2.12}
    $(-1,5, -0,7)$
  
\end{reponse}
\begin{reponse}{2.13}
    \begin{inparaenum}
    \item $\hat{\beta}_0 = 9,273$, $\hat{\beta}_1 = 1,436$
    \item $t = 9,809$
    \item $(1,105, 1,768)$
    \end{inparaenum}
  
\end{reponse}
\begin{reponse}{2.14}
    $F = 0,73$, valeur $p$: $0,397$
  
\end{reponse}
\begin{reponse}{2.15}
    $\hat{Y}_0 \pm t_{\alpha/2}(n - 1)\, s\,
    \sqrt{1 + X_0^2/\sum_{t=1}^n X_t^2}$
  
\end{reponse}
\begin{reponse}{2.16}
    \begin{inparaenum}
    \item $\text{PNB} = 1,168 + 1,716 \text{ MM}$
    \item $\beta_0 \in (0,060, 2,276)$, $\beta_1 \in (1,427, 2,005)$
    \item $6,31$
    \item $(11,20, 12,80)$ et $(10,83, 13,17)$
    \end{inparaenum}
  
\end{reponse}
\begin{reponse}{2.18}
    \begin{inparaenum}
      \stepcounter{enumi}
    \item $R^2 = 0,858$ et
      $F = 217,5$
    \item $10,57 \pm
      2,13$
    \end{inparaenum}
  
\end{reponse}
